internal/examples/semantics/structs.go
@@ -1,0 +1,89 @@
+package semantics
+
+// helpers
+type TwoInts struct {
+	x uint64
+	y uint64
+}
+
+type S struct {
+	a uint64
+	b TwoInts
+	c bool
+}
+
+func NewS() *S {
+	return &S{
+		a: 2,
+		b: TwoInts{x: 1, y: 2},
+		c: true,
+	}
+}
+
+func (s *S) readA() uint64 {
+	return s.a
+}
+
+func (s *S) readB() TwoInts {
+	return s.b
+}
+
+func (s S) readBVal() TwoInts {
+	return s.b
+}
+
+func (s *S) updateBValX(i uint64) {
+	s.b.x = i
+}
+
+func (s *S) negateC() {
+	s.c = !s.c
+}
+
+// tests
+func failing_testStructUpdates() bool {
+	var ok = true
+	var ns = NewS()
+
+	ok = ok && (ns.readA() == 2)
+	var b1 = ns.readB()
+	ok = ok && (b1.x == 1)
+	ns.negateC()
+	ok = ok && (ns.c == false)
+
+	b1.x = 3
+	var b2 = ns.readB()
+	ok = ok && (b2.x == 1)
+
+	var b3 = &ns.b
+	ok = ok && b3.x == 1
+
+	ns.updateBValX(4)
+	ok = ok && (ns.readBVal().x == 4)
+	return ok
+}
+
+func failing_testNestedStructUpdate() bool {
+	var ns = NewS()
+	ns.b.x = 5
+	return ns.b.x == 5
+}
+
+func testStructConstructions() bool {
+	var ok = true
+
+	var p1 *TwoInts           // p1 == nil
+	var p2 TwoInts            // p2 == TwoInts{0, 0}
+	p3 := TwoInts{y: 0, x: 0} // p3 == TwoInts{0, 0}
+	p4 := TwoInts{x: 0, y: 0} // p4 == TwoInts{0, 0}
+
+	ok = ok && (p1 == nil)
+	p1 = new(TwoInts) // p1 == &TwoInts{0, 0}
+
+	ok = ok && (p2 == p3)
+	ok = ok && (p3 == p4)
+	ok = ok && (p4 == *p1)
+
+	ok = ok && (&p4 != p1)
+	return ok
+}
